Makefile
@@ -12,14 +12,20 @@ CLIGHTGEN?=clightgen
 -include CONFIGURE
 
 COQLIB=$(shell $(COQC) -where | tr -d '\r' | tr '\\' '/')
+COQLIBINSTALL=$(COQLIB)/user-contrib
 ifeq ($(BITSIZE),64)
 	COMPCERT_DIR=$(COQLIB)/user-contrib/compcert
 	VST_DIR=$(COQLIB)/user-contrib/VST
+	CERTIGRAPH_DIR=$(COQLIB)/user-contrib/CertiGraph
 else ifeq ($(BITSIZE),32)
+	CLIGHTGEN=$(COQLIB)/../../variants/compcert32/bin/clightgen
+	COQLIBINSTALL=$(COQLIB)/../coq-variant/CertiGC32
 	COMPCERT_DIR=$(COQLIB)/../coq-variant/compcert32/compcert
 	VST_DIR=$(COQLIB)/../coq-variant/VST32/VST
-	CLIGHTGEN=$(COQLIB)/../../variants/compcert32/bin/clightgen
+	CERTIGRAPH_DIR=$(COQLIB)/../coq-variant/CertiGraph32/CertiGraph
 endif
+
+INSTALLDIR?=$(COQLIBINSTALL)/CertiGC
 
 TARGET=x86_64-linux
 ifeq ($(BITSIZE),32)
@@ -28,20 +34,23 @@ endif
 
 
 src/ast/x86_64-linux/gc.v: c/gc.c c/gc.h c/config.h c/mem.h
+	mkdir -p src/ast/x86_64-linux
 	$(CLIGHTGEN) -Wall -Wno-unused-variable -Werror -normalize c/gc.c -o src/ast/x86_64-linux/gc.v
 
 src/ast/x86_32-linux/gc.v: c/gc.c c/gc.h c/config.h c/mem.h
+	mkdir -p src/ast/x86_32-linux
 	$(CLIGHTGEN) -Wall -Wno-unused-variable -Werror -normalize c/gc.c -o src/ast/x86_32-linux/gc.v
 
 _CoqProject: src/ast/$(TARGET)/gc.v
-	echo "-Q src/ast CertiGC.ast"                           		> $@
-	echo "-Q src/ast/$(TARGET) CertiGC.ast.clightgen"    			>> $@
-	echo "-Q src/model CertiGC.model"                       		>> $@
-	echo "-Q src/proof CertiGC.proof"                       		>> $@
-	echo "-Q src/spec CertiGC.spec"                         		>> $@
-	@[ -z $(VST_DIR) ] 		|| echo "-Q $(VST_DIR) VST" 			>> $@
-	@[ -z $(COMPCERT_DIR) ] || echo "-Q $(COMPCERT_DIR) compcert"	>> $@
-	find ./ -name "*.v" | cut -d'/' -f2-                    		>> $@
+	echo "-Q src/ast CertiGC.ast"                           				> $@
+	echo "-Q src/ast/$(TARGET) CertiGC.ast.clightgen"    					>> $@
+	echo "-Q src/model CertiGC.model"                       				>> $@
+	echo "-Q src/proof CertiGC.proof"                       				>> $@
+	echo "-Q src/spec CertiGC.spec"                         				>> $@
+	@[ -z $(VST_DIR) ] 			|| echo "-Q $(VST_DIR) VST" 				>> $@
+	@[ -z $(COMPCERT_DIR) ] 	|| echo "-Q $(COMPCERT_DIR) compcert"		>> $@
+	@[ -z $(CERTIGRAPH_DIR) ]	|| echo "-Q $(CERTIGRAPH_DIR) CertiGraph"	>> $@
+	find ./ -name "*.v" | cut -d'/' -f2-                    				>> $@
 
 Makefile.coq: Makefile _CoqProject
 	coq_makefile -f _CoqProject -o Makefile.coq
@@ -49,8 +58,18 @@ Makefile.coq: Makefile _CoqProject
 theories: Makefile.coq
 	$(MAKE) -f Makefile.coq -j$(J)
 
+
+C_SOURCES=$(shell find ./ -name "*.c" | cut -d'/' -f2-) $(shell find ./ -name "*.h" | cut -d'/' -f2-)
+COQ_SOURCES=$(shell find ./ -name "*.v" | cut -d'/' -f2-)
+
+INSTALL_SOURCES=$(C_SOURCES) $(COQ_SOURCES)
+INSTALL_COMPILED=$(COQ_SOURCES:%.v=%.vo)
+
+.PHONY: install
 install:
-	echo "TODO! ;0"
+	install -d "$(INSTALLDIR)"
+	for d in $(sort $(dir $(INSTALL_SOURCES) $(INSTALL_COMPILED))); do install -d "$(INSTALLDIR)/$$d"; done
+	for f in $(INSTALL_SOURCES) $(INSTALL_COMPILED); do install -m 0644 $$f "$(INSTALLDIR)/$$(dirname $$f)"; done
 
 clean:
 	[ ! -f Makefile.coq ] || $(MAKE) -f Makefile.coq clean
@@ -59,6 +78,8 @@ clean:
 	rm -f `find ./ -name "*.aux"`
 	rm -f `find ./ -name "*.glob"`
 	rm -f `find ./ -name "*.vo*"`
+	rm -rf src/ast/x86_32-linux
+	rm -rf src/ast/x86_64-linux
 
 deepclean: clean
 	rm -f _CoqProject
